before deleting fidelity stuff

lemma/live_proc.v
@@ -4,17 +4,15 @@ Import ListNotations.
 Open Scope list_scope.
 From Paco Require Import paco.
 Import ListNotations. 
-
 From SST Require Import src.header src.sim src.expr src.process src.local 
 src.global src.balanced src.typecheck src.part src.gttreeh src.path_props src.step src.merge src.projection src.session src.lcontext.  
 From SST Require Import lemma.inversion lemma.inversion_expr lemma.completeness lemma.substitution_helper lemma.substitution lemma.decidable_helper lemma.decidable lemma.expr lemma.part lemma.step 
 lemma.projection_helper lemma.subj_red_prog lemma.projection lemma.main_helper lemma.soundness lemma.liveness_helpers. 
 
-Definition betaRtc := clos_refl_trans session betaP.
-Check p_send.
-Check typ_sess.
-
-Check guardP_break.
+Inductive betaRtc : session -> session -> Prop:=
+    | betaRt_unf : forall a b, unfoldP a b -> betaRtc a b
+    | betaRt_beta : forall a b, betaP a b -> betaRtc a b
+    | betaRtrans : forall a b c, betaRtc a b -> betaRtc b c -> betaRtc a c.
 
 Definition all_guarded P := forall n, exists m, guardP n m P.
 
@@ -54,75 +52,205 @@ Qed.
 
 Hint Resolve betaPr_unfold_one :procs.
 
-Lemma inv_proc_send : forall M gamma p q xsp, typ_sess M gamma ->
-M.find p gamma = Some (ltt_send q xsp) -> exists M' M'' P' e ell,
-betaRtc M M' /\ 
-unfoldP M' ((p <-- p_send q ell e P')||| M'').
+Definition betaPtrans := clos_trans process  betaPr. 
+
+Check guardP_break.
+
+Inductive is_ite_or_send : process -> Prop :=
+    | ite_send_send: forall q ell e P', is_ite_or_send (p_send q ell e P')
+    | ite_send_rec: forall P P',  betaPtrans (p_rec P) P' -> is_ite_or_send P' -> is_ite_or_send (p_rec P)
+    | ite_send_ite : forall e P1 P2, is_ite_or_send P1 -> is_ite_or_send P2 -> is_ite_or_send (p_ite e P1 P2).
+
+Search (relation _ -> relation _ -> relation _) .
+
+Lemma betaRtc_stronger : forall a b, multi betaP a b -> betaRtc a b.
 Proof.
-    intros * Hsess Hfindp.
-    assert(Hinp:InT p M) by (
-    inversion Hsess;subst;eapply H0;red;exists (ltt_send q xsp);split;easy).
-    eapply move_forward_h in Hinp as Hmf.
-    destruct Hmf.
+    intros.
+    induction H. constructor. eauto with procs.
+    econstructor 3;try exact IHmulti. constructor 2. easy.
+Qed.
+
+Lemma betaPrtrans_implies_multi : forall a b, betaPtrans a b -> multi betaPr a b.
+Proof.
+    intros.
+    induction H;subst. econstructor 2;try exact H;try constructor.
+    eapply transitive_multi;try exact IHclos_trans1;easy.
+Qed.
+
+Hint Resolve betaPrtrans_implies_multi :procs.
+
+Theorem is_ite_implies_beta_send : forall M  p  P Tp, 
+is_ite_or_send P -> typ_proc [] [] P Tp -> exists q ell e P',
+    betaRtc (p <-- P ||| M) (p <-- p_send q ell e P' ||| M).
+Proof.
+    intros * Hite Htyp. induction Hite.
     {
-        destruct H as [P [M' Hunf]].
-        eapply typ_after_unfold in Hsess as Hsess';try exact Hunf.
-        assert(Hprocs  :typ_proc [] [] P (ltt_send q xsp) /\
-        (forall n : opt_lbl, exists m : opt_lbl, guardP n m P)).
-        {
-            inversion Hsess';subst.
-        
-            inversion_clear H2;subst;inversion_clear H3. destr_hyps.
-            clear H4 H1 H0.
-            rewrite Hfindp in H2;inversion H2;subst;clear H2. tauto.
-        }
-        destruct Hprocs as [Hproc Hguard].
-        eapply guardP_break in Hguard as Htr;destr_hyps. rename H into Punf.
-        eapply typ_proc_after_betaPr in Punf as Htyp';try exact Hproc.
-        rename H0 into Htr.
-        generalize dependent M.
-        pose proof Htyp' as Htyp.
-        generalize dependent P. 
-        dependent induction Htyp'.
-        {
-            intros.
-            destruct Htr as [Hu | [Hu | [Hu | Hu]]];destr_hyps;subst;easy. 
-        }
-        {
-            intros.
-            destruct Htr as [Hu | [Hu | [Hu | Hu]]];destr_hyps;subst;easy. 
-        }
-        {
-            intros. eapply inv_proc_ite in Htyp;try reflexivity;destr_hyps.
-            assert(Hguard1: all_guarded p1).
-            {
-                eapply guarded_after_multi_unfold in Punf;try exact Hguard.
-                eapply guard_ite_inv in Punf;try easy.
-            }
-            assert(Hguard2: all_guarded p2).
-            {
-                eapply guarded_after_multi_unfold in Punf;try exact Hguard.
-                eapply guard_ite_inv in Punf;try easy.
-            }
-            eapply guardP_break in Hguard1 as [P1 Hbre1]. 
-            eapply guardP_break in Hguard2 as [P2 Hbre2].
-            assert (Hnp: unfoldP M ((p <-- p_ite e p1 p2) ||| M')).
-            {
-                destr_hyps.   
-                eauto with procs.
-            }
-            eapply expr_eval_b in H4. destruct H4.
-            
-
-            assert(Hbet: betaP ((p <-- p_ite e p1 p2) ||| M') ((p <-- p1) ||| M'))
-            by (eapply rt_ite;easy).
-            eapply IHHtyp'1 with (P:=P1) (M:=((p <-- P1) ||| M')) in Hfindp as IH_use; try easy. 
-            admit. right.
-        }
-
-        induction Punf.
-        assert(typ_proc [] [] )
+     exists q, ell ,e, P'.  constructor. eauto with procs.      
     }
+    {
+        destr_hyps.
+        
+        eapply typ_proc_after_betaPr in Htyp;try exact H. specialize (IHHite Htyp).
+        destr_hyps. 
+        
+        exists x, x0, x1, x2. econstructor 3;try exact H0. constructor 1. 
+        1-2: eauto with procs. 
+    }
+    {
+        eapply typable_implies_wfC in Htyp as Hwfc.   
+        eapply inv_proc_ite in Htyp;try reflexivity. destr_hyps.
+        assert(typ_proc [] [] P1 Tp). eapply tc_sub;try exact H;try easy.
+        
+        assert(typ_proc [] [] P2 Tp). eapply tc_sub;try exact H0;try easy.
+        specialize (IHHite1 H4).
+        specialize (IHHite2 H5).
+        eapply expr_eval_b in H3. destruct H3.
+        {
+            assert(betaP ((p <-- p_ite e P1 P2) ||| M) ((p <-- P1 ) ||| M)) by (constructor;easy).
+            destr_hyps. exists x5, x6, x7, x8.
+            eapply betaRt_beta in H6.
+            econstructor 3; try exact H6. easy.   
+        }
+        {
+         
+            assert(betaP ((p <-- p_ite e P1 P2) ||| M) ((p <-- P2) ||| M)) by (constructor;easy).
+            destr_hyps. exists x1, x2, x3, x4.
+            eapply betaRt_beta in H6.
+            econstructor 3; try exact H6. easy.   
+        }
+
+    }
+Qed.
+
+Lemma betaPr_unique : forall a b c, betaPr a b -> betaPr a c -> b=c.
+        intros. inversion H;inversion H0;subst.
+        inversion H5;subst.
+        eapply substitution_helper.inj_substP in H1;try exact H4;subst;easy.
+Qed.
+
+Lemma betaPr_factor : forall a b c, betaPr a b -> betaPtrans a c -> 
+(betaPtrans b c  \/ b=c).
+Proof.
+    intros.
+    induction H0;intros;try tauto.
+    {
+        eapply betaPr_unique in H;try exact H0;subst;tauto.
+    }
+    {
+        specialize (IHclos_trans1 H). destruct IHclos_trans1.
+        left. econstructor 2;try exact H0_0. easy.
+        subst. left. easy.   
+    }
+Qed.
+
+Lemma betaPr_linear : forall a b c, betaPtrans a b -> betaPtrans a c -> 
+(betaPtrans b c  \/ betaPtrans c b \/ b=c).
+Proof.
+    intros.
+    induction H;intros;try tauto.
+    {
+        eapply betaPr_factor in H0;try exact H. tauto.
+    }
+    {
+        specialize (IHclos_trans1 H0). destruct IHclos_trans1.
+        eapply IHclos_trans2;easy.
+
+        destruct H2;subst. right. left. econstructor 2;try exact H1;easy.
+        right. left. easy.   
+    }
+Qed.
+
+Lemma betaPr_trans_form : forall x y, betaPtrans x y -> exists z, x=p_rec z.
+Proof.
+    intros. induction H.
+    inversion H;subst. exists P;easy.
+    destr_hyps;subst. exists x1. easy.
+Qed.
+
+Lemma is_ite_or_send_betaPr : forall P Q, is_ite_or_send P -> betaPtrans P Q ->
+is_ite_or_send Q.
+Proof.
+    intros * Hite. generalize dependent Q. 
+    induction Hite;intros * Hunf;try solve [inversion Hunf].
+    {
+        eapply betaPr_trans_form in Hunf;destr_hyps;subst;easy.
+    }
+    {   
+        eapply betaPr_linear in Hunf as Hdil;try exact H.
+        destruct Hdil.
+        {
+         
+            eapply IHHite;easy.
+        }
+        destruct H0;subst.
+        eapply betaPr_trans_form in H0 as Ht;destr_hyps;subst.
+        econstructor 2;try exact H0;try easy.
+        easy.
+    }
+    {
+     eapply betaPr_trans_form in Hunf;destr_hyps;subst;easy.
+    }
+Qed.
+
+Theorem typ_send_means_ite_or_send :  forall   P gs gt q xsp, 
+typ_proc gs gt P (ltt_send q xsp) -> is_ite_or_send P.
+Proof.
+    induction P;intros.
+    { constructor.   
+    }
+    {
+        eapply inv_proc_recv in H;try reflexivity;destr_hyps. pinversion H0;try apply sub_mon.       
+    }
+    {
+        eapply typable_implies_wfC in H as Hwfc.
+        eapply inv_proc_ite in H;try reflexivity;destr_hyps.
+        
+        eapply tc_sub in H;try exact H1;try easy.
+        eapply tc_sub in H0;try exact H2;try easy.
+        constructor. eapply IHP1;try exact H.
+        eapply IHP2;try exact H0.   
+    }
+    {
+        
+        eapply typable_implies_wfC in H as Hwfc.
+        eapply inv_proc_rec in H;try reflexivity;destr_hyps.
+        eapply tc_sub in H;try exact H0;try easy.
+        
+        
+
+        Lemma is_ite_guarded : forall P Q R, all_guarded (p_rec P) -> 
+        substitutionP 0 0 0 R P Q -> 
+        is_ite_or_send Q -> is_ite_or_send P.
+        Proof.
+            intros. 
+            generalize dependent Q.
+            generalize dependent R.
+            induction P;intros.
+            { 
+                constructor.   
+            }
+            {
+                inversion H0;subst. inversion H1.   
+            }
+            {
+                constructor;
+                inversion H0;subst;
+                inversion H1;subst.
+                eapply IHP1;try exact H10;try easy.
+                admit.
+                eapply IHP2;try exact H11;try easy.
+                admit. 
+            }
+            {
+                econstructor.   
+            }
+            econstructor;try*)
+        econstructor.
+        
+        eapply IHP in H.
+    }
+    intros.
+
 Theorem sess_fidelity : forall M gamma p q ell gamma', 
 typ_sess M gamma -> tctxR gamma (lcomm p q ell) gamma' ->
     exists gamma'' M', tctxR gamma (lcomm p q ell) gamma'' /\ betaRtc M M' /\ typ_sess M' gamma''.
@@ -138,6 +266,7 @@ Proof.
     {
         destruct Hcanon as [M' [P [Q Hunf]]].
         eapply typ_after_unfold in Hunf as Hsess';try exact Hsess.
+       
         clear x H H1 Htwf Hin Hndup Hfat. 
         inversion Hsess';subst. destruct Hassocable as [g [Hwfg Hassoc]].
         rename H into Htwf, H1 into Hinend, H8 into Hnodup, H9 into Hfat.
@@ -145,70 +274,46 @@ Proof.
         inversion_clear H9. destr_hyps.
         rewrite H0 in H;inversion H;subst.
         rewrite H2 in H8;inversion H8;subst;clear H H8.
+        generalize dependent M.
+        induction P. 1-2:admit.
+        {
+            eapply inv_proc_ite in H11 as Hite;try reflexivity;destr_hyps.
+            eapply expr_eval_b in H15.
+            destruct H15;try easy.
+            {
+                intros.
+                
+                assert(Hbet: betaP ((p <-- p_ite e P1 P2) ||| ((q <-- Q) ||| M')) 
+                ((p <-- P1 ) ||| ((q <-- Q) ||| M'))) by (constructor;try easy).
+                assert(Hunf': unfoldP M ((p <-- p_ite e P1 P2) ||| ((q <-- Q) ||| M'))) by
+                eauto with procs.
+                assert(Hbet2 : betaP M ((p <-- P1) ||| ((q <-- Q) ||| M'))).
+                eapply r_struct;try exact Hbet;try easy;try constructor.
+                assert(unfoldP ((p <-- P1) ||| ((q <-- Q) ||| M')) ((p <-- P1) ||| ((q <-- Q) ||| M'))) by constructor.
+                admit.
+            }
+            admit.
+        }
+        {
+            intros.
+
+        }
+
         rename H11 into Htypp.
-        eapply guardP_break in H12. destruct H12 as [Punf [Hpunf Htr]].
-        eapply typ_proc_after_betaPr in Htypp as Htyp_unf;try exact Hpunf.
-        induction Punf.
+        induction P.
+        {
+            admit.      
+        }
         {
             admit.   
         }
         {
-            admit.
-        }
-        {
 
         }
-        (*evar (Cs: list (option sort)).
-        evar (Ct: list (option ltt)).
-        instantiate (Ct:=[]).
-        instantiate (Cs:=[]).
-        fold Cs in Htypp.
-        fold Ct in Htypp.
-        clearbody Cs Ct.
-        generalize dependent Cs.
-        generalize dependent Ct.
-        intros.
-        
-        clear H6 H7 x5 x3 x0 x1 H3 H4 H5.
-        rename x2 into xsp, x4 into xsq.
-        
-        remember (ltt_send q x2) as t_lbl.
-        pose proof Htypp as Htypp_rem.
 
-        induction Htypp;try easy.
-        {
-            
-            specialize (H12 1). destr_hyps. 
-            inversion H11;subst.
-        }
-        {
-            eapply guardP_break in H12.
-            destr_hyps. rename x into Punf.
-            destruct H8;subst.
-            { 
-                eapply typ_proc_after_betaPr in Htypp_rem;try exact H.
-                eapply inv_proc_inact in Htypp_rem;subst;try easy.
-            }
-            destruct H8.
-            {
-                destr_hyps;subst.
-                eapply typ_proc_after_betaPr in Htypp_rem;try exact H.
-                eapply inv_proc_ite in Htypp_rem;try reflexivity;destr_hyps;subst.
-                eapply IHHtypp  in Hsess as IH_use;try assumption.
-                all:try easy.
-                Print "~=".
-            }   
-        }
-        (*dep ind*)
         eapply guardP_break in H12. destruct H12 as [Punf [Hpunf Htr]].
         eapply typ_proc_after_betaPr in Htypp as Htyp_unf;try exact Hpunf.
-        (*evar (Cs: list (option sort)).
-        evar (Ct: list (option ltt)).
-        instantiate (Ct:=[]).
-        instantiate (Cs:=[]).
-        fold Cs in Htyp_unf.
-        fold Ct in Htyp_unf.
-        clearbody Cs Ct.*)
+        
         pose proof Htyp_unf as Htyp_unfr.
         dependent induction Htyp_unfr.
         {
@@ -217,15 +322,16 @@ Proof.
         {
             destruct Htr as [Hu | [Hu | [Hu | Hu]]];destr_hyps;subst;try easy.
         }
-        {   
-            eapply inv_proc_ite in Htyp_unf;try reflexivity;destr_hyps.
+        {
+
+            eapply inv_proc_ite in Htyp_unf as Hinv_ite;try reflexivity;destr_hyps.
             eapply expr_eval_b in H14.
             destruct H14.
             {
-                eapply IHHtyp_unfr1 with (q:=q) (x2:=x2) in H9 ;try easy.   
+
             }
             Search typ_expr sbool.
-        }*)
+        }
         
     }
     specialize (Hin p). unfold in_not_end in Hin.
